raft/RaftLinearizableDefinitions.v
@@ -1,0 +1,23 @@
+Require Import List.
+Import ListNotations.
+
+Require Import VerdiTactics.
+Require Import Util.
+Require Import Net.
+
+Require Import Raft.
+
+Section RaftLinearizableDefinitions.
+  Context {orig_base_params : BaseParams}.
+  Context {one_node_params : OneNodeParams orig_base_params}.
+  Context {raft_params : RaftParams orig_base_params}.
+
+  Definition project_input_keys (tr : list (name * (raft_input + list raft_output))) : list (nat * nat) :=
+    filterMap (fun x => match x with
+                          | (_, inl (ClientRequest client id _)) => Some (client, id)
+                          | _ => None
+                        end) tr.
+
+  Definition input_correct (tr : list (name * (raft_input + list raft_output))) : Prop :=
+    NoDup (project_input_keys tr).
+End RaftLinearizableDefinitions.
